src/ModularArithmetic/ModularBaseSystemOpt.v
@@ -4,8 +4,12 @@ Require Import Crypto.ModularArithmetic.PseudoMersenneBaseParamProofs.
 Require Import Crypto.ModularArithmetic.ModularBaseSystemProofs.
 Require Import Crypto.ModularArithmetic.ExtendedBaseVector.
 Require Import Crypto.ModularArithmetic.Pow2BaseProofs.
-Require Import Crypto.BaseSystem Crypto.ModularArithmetic.ModularBaseSystem.
+Require Import Crypto.BaseSystem.
+Require Import Crypto.ModularArithmetic.ModularBaseSystemList.
+Require Import Crypto.ModularArithmetic.ModularBaseSystemListProofs.
+Require Import Crypto.ModularArithmetic.ModularBaseSystem.
 Require Import Coq.Lists.List.
+Require Import Crypto.Util.Tuple.
 Require Import Crypto.Util.ListUtil Crypto.Util.ZUtil Crypto.Util.NatUtil Crypto.Util.CaseUtil.
 Import ListNotations.
 Require Import Coq.ZArith.ZArith Coq.ZArith.Zpower Coq.ZArith.ZArith Coq.ZArith.Znumtheory.
@@ -14,8 +18,7 @@ Require Import Crypto.Tactics.VerdiTactics.
 Local Open Scope Z.
 
 Class SubtractionCoefficient (m : Z) (prm : PseudoMersenneBaseParams m) := {
-  coeff : BaseSystem.digits;
-  coeff_length : (length coeff = length (Pow2Base.base_from_limb_widths limb_widths))%nat;
+  coeff : tuple Z (length limb_widths);
   coeff_mod: decode coeff = 0%F
 }.
 
@@ -37,9 +40,9 @@ Definition map_opt {A B} := Eval compute in @map A B.
 Definition full_carry_chain_opt := Eval compute in @Pow2Base.full_carry_chain.
 Definition length_opt := Eval compute in length.
 Definition base_from_limb_widths_opt := Eval compute in @Pow2Base.base_from_limb_widths.
-Definition max_ones_opt := Eval compute in @max_ones.
-Definition max_bound_opt := Eval compute in @max_bound.
 Definition minus_opt := Eval compute in minus.
+Definition max_ones_opt := Eval compute in @max_ones.
+Definition from_list_default_opt {A} := Eval compute in (@from_list_default A).
 
 Definition Let_In {A P} (x : A) (f : forall y : A, P y)
   := let y := x in f y.
@@ -110,14 +113,16 @@ Section Carries.
     (* allows caller to precompute k and c *)
     (k_ c_ : Z) (k_subst : k = k_) (c_subst : c = c_).
   Local Notation base := (Pow2Base.base_from_limb_widths limb_widths).
+  Local Notation digits := (tuple Z (length limb_widths)).
 
   Definition carry_opt_sig
              (i : nat) (b : digits)
     : { d : digits | (i < length limb_widths)%nat -> d = carry i b }.
   Proof.
     eexists ; intros.
-    cbv [carry].
-    rewrite <- pull_app_if_sumbool.
+    cbv [carry ModularBaseSystemList.carry].
+    rewrite <-from_list_default_eq with (d := 0%Z).
+    rewrite <-pull_app_if_sumbool.
     cbv beta delta
       [carry carry_and_reduce Pow2Base.carry_gen Pow2Base.carry_and_reduce_single Pow2Base.carry_simple
        Z.pow2_mod Z.ones Z.pred
@@ -127,12 +132,13 @@ Section Carries.
     change @nth_default with @nth_default_opt in *.
     change @set_nth with @set_nth_opt in *.
     lazymatch goal with
-    | [ |- _ = (if ?br then ?c else ?d) ]
+    | [ |- _ = _ (if ?br then ?c else ?d) ]
       => let x := fresh "x" in let y := fresh "y" in evar (x:digits); evar (y:digits); transitivity (if br then x else y); subst x; subst y
     end.
     2:cbv zeta.
     2:break_if; reflexivity.
 
+    change @from_list_default with @from_list_default_opt.
     change @nth_default with @nth_default_opt.
     rewrite c_subst.
     change @set_nth with @set_nth_opt.
@@ -141,10 +147,12 @@ Section Carries.
     reflexivity.
   Defined.
 
-  Definition carry_opt i b
-    := Eval cbv beta iota delta [proj1_sig carry_opt_sig] in proj1_sig (carry_opt_sig i b).
+  Definition carry_opt is us := Eval cbv [proj1_sig carry_opt_sig] in
+                                          proj1_sig (carry_opt_sig is us).
 
-  Definition carry_opt_correct i b : (i < length limb_widths)%nat -> carry_opt i b = carry i b := proj2_sig (carry_opt_sig i b).
+  Definition carry_opt_correct i us
+    : (i < length limb_widths)%nat -> carry_opt i us = carry i us
+    := proj2_sig (carry_opt_sig i us).
 
   Definition carry_sequence_opt_sig (is : list nat) (us : digits)
     : { b : digits | (forall i, In i is -> i < length base)%nat -> b = carry_sequence is us }.
@@ -183,8 +191,8 @@ Section Carries.
     cbv beta iota delta [carry_opt].
     let LHS := match goal with |- ?LHS = ?RHS => LHS end in
     let RHS := match goal with |- ?LHS = ?RHS => RHS end in
-    let RHSf := match (eval pattern (nth_default_opt 0%Z b i) in RHS) with ?RHSf _ => RHSf end in
-    change (LHS = Let_In (nth_default_opt 0%Z b i) RHSf).
+    let RHSf := match (eval pattern (nth_default_opt 0%Z (to_list _ b) i) in RHS) with ?RHSf _ => RHSf end in
+    change (LHS = Let_In (nth_default_opt 0%Z (to_list _ b) i) RHSf).
     change Z.shiftl with Z_shiftl_opt.
     change (-1) with (Z_opp_opt 1).
     change Z.add with Z_add_opt at 5 9 17 21.
@@ -265,13 +273,13 @@ Section Carries.
 
 
   Lemma carry_sequence_opt_cps_rep
-       : forall (is : list nat) (us : list Z) (x : F modulus),
+       : forall (is : list nat) (us : digits) (x : F modulus),
          (forall i : nat, In i is -> i < length base)%nat ->
          rep us x -> rep (carry_sequence_opt_cps is us) x.
   Proof.
     intros.
     rewrite carry_sequence_opt_cps_correct by assumption.
-    apply carry_sequence_rep; eauto using rep_length.
+    auto using carry_sequence_rep.
   Qed.
 
   Lemma full_carry_chain_bounds : forall i, In i (Pow2Base.full_carry_chain limb_widths) -> (i < length base)%nat.
@@ -320,6 +328,7 @@ End Carries.
 
 Section Addition.
   Context `{prm : PseudoMersenneBaseParams} {sc : SubtractionCoefficient modulus prm}.
+  Local Notation digits := (tuple Z (length limb_widths)).
 
   Definition add_opt_sig (us vs : digits) : { b : digits | b = add us vs }.
   Proof.
@@ -338,6 +347,7 @@ End Addition.
 
 Section Subtraction.
   Context `{prm : PseudoMersenneBaseParams} {sc : SubtractionCoefficient modulus prm}.
+  Local Notation digits := (tuple Z (length limb_widths)).
 
   Definition sub_opt_sig (us vs : digits) : { b : digits | b = sub coeff us vs }.
   Proof.
@@ -358,9 +368,11 @@ Section Multiplication.
   Context `{prm : PseudoMersenneBaseParams} {sc : SubtractionCoefficient modulus prm}
     (* allows caller to precompute k and c *)
     (k_ c_ : Z) (k_subst : k = k_) (c_subst : c = c_).
+  Local Notation digits := (tuple Z (length limb_widths)).
+
   Definition mul_bi'_step
-             (mul_bi' : nat -> digits -> list Z -> list Z)
-             (i : nat) (vsr : digits) (bs : list Z)
+             (mul_bi' : nat -> list Z -> list Z -> list Z)
+             (i : nat) (vsr : list Z) (bs : list Z)
     : list Z
     := match vsr with
        | [] => []
@@ -368,8 +380,8 @@ Section Multiplication.
        end.
 
   Definition mul_bi'_opt_step_sig
-             (mul_bi' : nat -> digits -> list Z -> list Z)
-             (i : nat) (vsr : digits) (bs : list Z)
+             (mul_bi' : nat -> list Z -> list Z -> list Z)
+             (i : nat) (vsr : list Z) (bs : list Z)
     : { l : list Z | l = mul_bi'_step mul_bi' i vsr bs }.
   Proof.
     eexists.
@@ -384,19 +396,19 @@ Section Multiplication.
   Defined.
 
   Definition mul_bi'_opt_step
-             (mul_bi' : nat -> digits -> list Z -> list Z)
-             (i : nat) (vsr : digits) (bs : list Z)
+             (mul_bi' : nat -> list Z -> list Z -> list Z)
+             (i : nat) (vsr : list Z) (bs : list Z)
     : list Z
     := Eval cbv [proj1_sig mul_bi'_opt_step_sig] in
         proj1_sig (mul_bi'_opt_step_sig mul_bi' i vsr bs).
 
   Fixpoint mul_bi'_opt
-           (i : nat) (vsr : digits) (bs : list Z) {struct vsr}
+           (i : nat) (vsr : list Z) (bs : list Z) {struct vsr}
     : list Z
     := mul_bi'_opt_step mul_bi'_opt i vsr bs.
 
   Definition mul_bi'_opt_correct
-             (i : nat) (vsr : digits) (bs : list Z)
+             (i : nat) (vsr : list Z) (bs : list Z)
     : mul_bi'_opt i vsr bs = mul_bi' bs i vsr.
   Proof.
     revert i; induction vsr as [|vsr vsrs IHvsr]; intros.
@@ -413,12 +425,12 @@ Section Multiplication.
   Qed.
 
   Definition mul'_step
-             (mul' : digits -> digits -> list Z -> digits)
-             (usr vs : digits) (bs : list Z)
-    : digits
+             (mul' : list Z -> list Z -> list Z -> list Z)
+             (usr vs : list Z) (bs : list Z)
+    : list Z
     := match usr with
        | [] => []
-       | u :: usr' => add (mul_each u (mul_bi bs (length usr') vs)) (mul' usr' vs bs)
+       | u :: usr' => BaseSystem.add (mul_each u (mul_bi bs (length usr') vs)) (mul' usr' vs bs)
        end.
 
   Lemma map_zeros : forall a n l,
@@ -428,9 +440,9 @@ Section Multiplication.
   Qed.
 
   Definition mul'_opt_step_sig
-             (mul' : digits -> digits -> list Z -> digits)
-             (usr vs : digits) (bs : list Z)
-    : { d : digits | d = mul'_step mul' usr vs bs }.
+             (mul' : list Z -> list Z -> list Z -> list Z)
+             (usr vs : list Z) (bs : list Z)
+    : { d : list Z | d = mul'_step mul' usr vs bs }.
   Proof.
     eexists.
     cbv [mul'_step].
@@ -449,18 +461,18 @@ Section Multiplication.
   Defined.
 
   Definition mul'_opt_step
-             (mul' : digits -> digits -> list Z -> digits)
-             (usr vs : digits) (bs : list Z)
-    : digits
+             (mul' : list Z -> list Z -> list Z -> list Z)
+             (usr vs : list Z) (bs : list Z)
+    : list Z
     := Eval cbv [proj1_sig mul'_opt_step_sig] in proj1_sig (mul'_opt_step_sig mul' usr vs bs).
 
   Fixpoint mul'_opt
-           (usr vs : digits) (bs : list Z)
-    : digits
+           (usr vs : list Z) (bs : list Z)
+    : list Z
     := mul'_opt_step mul'_opt usr vs bs.
 
   Definition mul'_opt_correct
-           (usr vs : digits) (bs : list Z)
+           (usr vs : list Z) (bs : list Z)
     : mul'_opt usr vs bs = mul' bs usr vs.
   Proof.
     revert vs; induction usr as [|usr usrs IHusr]; intros.
@@ -471,13 +483,17 @@ Section Multiplication.
       cbv [mul_each mul_bi].
       rewrite map_zeros.
       rewrite <- mul_bi'_opt_correct.
+      cbv [zeros].
       reflexivity. }
   Qed.
 
   Definition mul_opt_sig (us vs : digits) : { b : digits | b = mul us vs }.
   Proof.
     eexists.
-    cbv [BaseSystem.mul mul mul_each mul_bi mul_bi' zeros reduce].
+    cbv [mul ModularBaseSystemList.mul BaseSystem.mul mul_each mul_bi mul_bi' zeros reduce].
+    rewrite <- from_list_default_eq with (d := 0%Z).
+    change (@from_list_default Z) with (@from_list_default_opt Z).
+    apply f_equal.
     rewrite ext_base_alt.
     rewrite <- mul'_opt_correct.
     change @Pow2Base.base_from_limb_widths with base_from_limb_widths_opt.
@@ -525,8 +541,8 @@ Section with_base.
         int_width_pos : 0 < int_width;
         int_width_compat : forall w, In w limb_widths -> w <= int_width;
         c_pos : 0 < c;
-        c_reduce1 : c * (Z.ones (int_width - log_cap (pred (length base)))) < max_bound 0 + 1;
-        c_reduce2 : c <= max_bound 0 - c;
+        c_reduce1 : c * (Z.ones (int_width - log_cap (pred (length base)))) < 2 ^ log_cap 0;
+        c_reduce2 : c < 2 ^ log_cap 0 - c;
         two_pow_k_le_2modulus : 2 ^ k <= 2 * modulus
       }.
 End with_base.
@@ -538,29 +554,25 @@ Section Canonicalization.
     (* allows caller to precompute k and c *)
     (k_ c_ : Z) (k_subst : k = k_) (c_subst : c = c_)
     {int_width} (preconditions : freezePreconditions prm int_width).
+  Local Notation digits := (tuple Z (length limb_widths)).
+
+  Definition encodeZ_opt := Eval compute in Pow2Base.encodeZ.
 
   Definition modulus_digits_opt_sig :
-    { b : digits | b = modulus_digits }.
+    { b : list Z | b = modulus_digits }.
   Proof.
     eexists.
-    cbv beta iota delta [modulus_digits modulus_digits' app].
-    change @max_bound with max_bound_opt.
-    rewrite c_subst.
-    change length with length_opt.
-    change minus with minus_opt.
-    change Z.add with Z_add_opt.
-    change Z.sub with Z_sub_opt.
-    change @Pow2Base.base_from_limb_widths with base_from_limb_widths_opt.
+    cbv beta iota delta [modulus_digits].
+    change Pow2Base.encodeZ with encodeZ_opt.
     reflexivity.
   Defined.
 
-  Definition modulus_digits_opt : digits
+  Definition modulus_digits_opt : list Z
     := Eval cbv [proj1_sig modulus_digits_opt_sig] in proj1_sig (modulus_digits_opt_sig).
 
   Definition modulus_digits_opt_correct
     : modulus_digits_opt = modulus_digits
     := proj2_sig (modulus_digits_opt_sig).
-
 
   Definition carry_full_3_opt_cps_sig
              {T} (f : digits -> T)
@@ -587,20 +599,20 @@ Section Canonicalization.
     { b : digits | b = freeze us }.
   Proof.
     eexists.
-    cbv [freeze].
-    cbv [and_term].
+    cbv [freeze conditional_subtract_modulus].
+    rewrite <-from_list_default_eq with (d := 0%Z).
+    change (@from_list_default Z) with (@from_list_default_opt Z).
     let LHS := match goal with |- ?LHS = ?RHS => LHS end in
     let RHS := match goal with |- ?LHS = ?RHS => RHS end in
-    let RHSf := match (eval pattern (isFull (carry_full (carry_full (carry_full us)))) in RHS) with ?RHSf _ => RHSf end in
-    change (LHS = Let_In (isFull(carry_full (carry_full (carry_full us)))) RHSf).
+    let RHSf := match (eval pattern (to_list (length limb_widths) (carry_full (carry_full (carry_full us)))) in RHS) with ?RHSf _ => RHSf end in
+    change (LHS = Let_In (to_list (length limb_widths)  (carry_full (carry_full (carry_full us)))) RHSf).
     let LHS := match goal with |- ?LHS = ?RHS => LHS end in
     let RHS := match goal with |- ?LHS = ?RHS => RHS end in
     let RHSf := match (eval pattern (carry_full (carry_full (carry_full us))) in RHS) with ?RHSf _ => RHSf end in
     rewrite <-carry_full_3_opt_cps_correct with (f := RHSf).
-    cbv beta iota delta [and_term isFull isFull'].
+    cbv beta iota delta [ge_modulus ge_modulus'].
     change length with length_opt.
-    change @max_bound with max_bound_opt.
-    rewrite c_subst.
+    change (nth_default 0 modulus_digits) with (nth_default_opt 0 modulus_digits_opt).
     change @max_ones with max_ones_opt.
     change @Pow2Base.base_from_limb_widths with base_from_limb_widths_opt.
     change minus with minus_opt.
@@ -616,7 +628,7 @@ Section Canonicalization.
   Definition freeze_opt_correct us
     : freeze_opt us = freeze us
     := proj2_sig (freeze_opt_sig us).
-
+(*
   Lemma freeze_opt_canonical: forall us vs x,
     @pre_carry_bounds _ _ int_width us -> rep us x ->
     @pre_carry_bounds _ _ int_width vs -> rep vs x ->
@@ -643,5 +655,5 @@ Section Canonicalization.
     split; eauto using freeze_opt_canonical.
     auto using freeze_opt_preserves_rep.
   Qed.
-
+*)
 End Canonicalization.
