src/ModularArithmetic/ModularBaseSystemListProofs.v
@@ -1,0 +1,95 @@
+Require Import Zpower ZArith.
+Require Import Coq.Numbers.Natural.Peano.NPeano.
+Require Import List.
+Require Import VerdiTactics.
+Require Import Crypto.BaseSystemProofs.
+Require Import Crypto.ModularArithmetic.Pow2Base.
+Require Import Crypto.ModularArithmetic.Pow2BaseProofs.
+Require Import Crypto.ModularArithmetic.ExtendedBaseVector.
+Require Import Crypto.ModularArithmetic.PrimeFieldTheorems.
+Require Import Crypto.ModularArithmetic.PseudoMersenneBaseParams.
+Require Import Crypto.ModularArithmetic.PseudoMersenneBaseParamProofs.
+Require Import Crypto.Util.Tactics.
+Require Import Crypto.Util.ListUtil.
+Require Import Crypto.Util.Notations.
+
+Require Import Crypto.ModularArithmetic.ModularBaseSystemList.
+Local Open Scope Z_scope.
+
+Section LengthProofs.
+  Context `{prm :PseudoMersenneBaseParams}.
+  Local Notation base := (base_from_limb_widths limb_widths).
+
+  Lemma length_encode {x} : length (encode x) = length limb_widths.
+  Proof.
+    cbv [encode encodeZ]; intros.
+    rewrite encode'_spec;
+      auto using encode'_length, limb_widths_nonneg, Nat.eq_le_incl, base_length.
+  Qed.
+
+  Lemma length_reduce : forall us,
+      (length limb_widths <= length us <= length ext_base)%nat ->
+      (length (reduce us) = length limb_widths)%nat.
+  Proof.
+    rewrite extended_base_length.
+    unfold reduce; intros.
+    rewrite add_length_exact.
+    pose proof base_length.
+    rewrite map_length, firstn_length, skipn_length, Min.min_l, Max.max_l;
+      omega.
+  Qed.
+
+  Lemma length_mul {u v} :
+      length u = length limb_widths
+      -> length v = length limb_widths
+      -> length (mul u v) = length limb_widths.
+  Proof.
+    cbv [mul]; intros.
+    apply length_reduce.
+    destruct u; try congruence.
+    + rewrite @nil_length0 in *; omega.
+    + rewrite mul_length_exact, extended_base_length, base_length; try omega.
+      congruence.
+  Qed.
+
+  Section Sub.
+  Context {mm : list Z} (mm_length : length mm = length limb_widths).
+
+  Lemma length_sub {u v} :
+      length u = length limb_widths
+      -> length v = length limb_widths
+      -> length (sub mm u v) = length limb_widths.
+  Proof.
+    cbv [sub]; intros.
+    rewrite sub_length, add_length_exact.
+    repeat rewrite Max.max_r; omega.
+  Qed.
+  End Sub.
+
+  Lemma length_carry_and_reduce {us}: forall i, length (carry_and_reduce i us) = length us.
+  Proof. intros; unfold carry_and_reduce; autorewrite with distr_length; reflexivity. Qed.
+  Hint Rewrite @length_carry_and_reduce : distr_length.
+
+  Lemma length_carry {u i} :
+    length u = length limb_widths
+    -> length (carry i u) = length limb_widths.
+  Proof. intros; unfold carry; break_if; autorewrite with distr_length; omega. Qed.
+  Hint Rewrite @length_carry : distr_length.
+
+  Lemma length_modulus_digits : length modulus_digits = length limb_widths.
+  Proof.
+    intros; unfold modulus_digits, encodeZ.
+    rewrite encode'_spec, encode'_length;
+      auto using encode'_length, limb_widths_nonneg, Nat.eq_le_incl, base_length.
+  Qed.
+
+  Lemma length_conditional_subtract_modulus {u cond} :
+    length u = length limb_widths
+    -> length (conditional_subtract_modulus u cond) = length limb_widths.
+  Proof.
+    intros; unfold conditional_subtract_modulus.
+    rewrite map2_length, map_length, length_modulus_digits.
+    apply Min.min_case; omega.
+  Qed.
+
+End LengthProofs.
